{
"cells": [
{"cell_type":    "code", "execution_count":null, "metadata":{}, "source":["%%html\n<link href=\"https:\/\/pretextbook.org\/beta\/mathbook-content.css\" rel=\"stylesheet\" type=\"text\/css\" \/>\n<link href=\"https:\/\/aimath.org\/mathbook\/mathbook-add-on.css\" rel=\"stylesheet\" type=\"text\/css\" \/>\n<link href=\"https:\/\/fonts.googleapis.com\/css?family=Open+Sans:400,400italic,600,600italic\" rel=\"stylesheet\" type=\"text\/css\" \/>\n<link href=\"https:\/\/fonts.googleapis.com\/css?family=Inconsolata:400,700&subset=latin,latin-ext\" rel=\"stylesheet\" type=\"text\/css\" \/><!-- Hide this cell. -->\n<script>\nvar cell = $(\".container .cell\").eq(0), ia = cell.find(\".input_area\")\nif (cell.find(\".toggle-button\").length == 0) {\nia.after(\n    $('<button class=\"toggle-button\">Toggle hidden code<\/button>').click(\n        function (){ ia.toggle() }\n        )\n    )\nia.hide()\n}\n<\/script>\n"], "outputs":[]},
{"cell_type":"markdown", "metadata":{}, "source":["**Important:** to view this notebook properly you will need to execute the cell above, which assumes you have an Internet connection.  It should already be selected, or place your cursor anywhere above to select.  Then press the \"Run\" button in the menu bar above (the right-pointing arrowhead), or press Shift-Enter on your keyboard."]},
{"cell_type":"markdown", "metadata":{}, "source":["$\\newcommand{\\spn}{\\operatorname{span}}\n\\newcommand{\\bbm}{\\begin{bmatrix}}\n\\newcommand{\\ebm}{\\end{bmatrix}}\n\\newcommand{\\R}{\\mathbb{R}}\n\\renewcommand{\\C}{\\mathbb{C}}\n\\newcommand{\\im}{\\operatorname{im}}\n\\newcommand{\\nll}{\\operatorname{null}}\n\\newcommand{\\csp}{\\operatorname{col}}\n\\newcommand{\\rank}{\\operatorname{rank}}\n\\newcommand{\\diag}{\\operatorname{diag}}\n\\newcommand{\\tr}{\\operatorname{tr}}\n\\newcommand{\\dotp}{\\!\\boldsymbol{\\cdot}\\!}\n\\newcommand{\\len}[1]{\\lVert #1\\rVert}\n\\newcommand{\\abs}[1]{\\lvert #1\\rvert}\n\\newcommand{\\proj}[2]{\\operatorname{proj}_{#1}{#2}}\n\\newcommand{\\bz}{\\overline{z}}\n\\newcommand{\\zz}{\\mathbf{z}}\n\\newcommand{\\uu}{\\mathbf{u}}\n\\newcommand{\\vv}{\\mathbf{v}}\n\\newcommand{\\ww}{\\mathbf{w}}\n\\newcommand{\\xx}{\\mathbf{x}}\n\\newcommand{\\yy}{\\mathbf{y}}\n\\newcommand{\\zer}{\\mathbf{0}}\n\\newcommand{\\basis}[2]{\\{\\mathbf{#1}_1,\\mathbf{#1}_2,\\ldots,\\mathbf{#1}_{#2}\\}}\n\\newcommand{\\gt}{>}\n\\newcommand{\\amp}{&}\n$"]},
{"cell_type":"markdown", "metadata":{}, "source":["<div class=\"mathbook-content\"><h6 class=\"heading hide-type\"><span xmlns:svg=\"http:\/\/www.w3.org\/2000\/svg\" class=\"type\">Section<\/span> <span class=\"codenumber\">5.2<\/span> <span class=\"title\">The matrix of a linear operator<\/span><\/h6><\/div>"]},
{"cell_type":"markdown", "metadata":{}, "source":["<div class=\"mathbook-content\"><p xmlns:svg=\"http:\/\/www.w3.org\/2000\/svg\" id=\"p-657\">Recall that a linear transformation $T:V\\to V$ is referred to as a <dfn class=\"terminology\">linear operator<\/dfn>. Recall also that two matrices $A$ and $B$ are <dfn class=\"terminology\">similar<\/dfn> if there exists an invertible matrix $P$ such that $B = PAP^{1-}\\text{,}$ and that similar matrices have a lot of properties in common. In particular, if $A$ is similar to $B\\text{,}$ then $A$ and $B$ have the same trace, determinant, and eigenvalues. One way to understand this is the realization that two matrices are similar if they are representations of the <em class=\"emphasis\">same<\/em> operator, with respect to <em class=\"emphasis\">different<\/em> bases.<\/p><\/div>"]},
{"cell_type":"markdown", "metadata":{}, "source":["<div class=\"mathbook-content\"><p xmlns:svg=\"http:\/\/www.w3.org\/2000\/svg\" id=\"p-658\">Since the domain and codomain of a linear operator are the same, we can consider the matrix $M_{DB}(T)$ where $B$ and $D$ are the <em class=\"emphasis\">same<\/em> ordered basis. This leads to the next definition.<\/p><\/div>"]},
{"cell_type":"markdown", "metadata":{}, "source":["<div class=\"mathbook-content\"><article class=\"definition definition-like\" id=\"def-operator-matrix\"><h6 xmlns:svg=\"http:\/\/www.w3.org\/2000\/svg\" class=\"heading\"><span class=\"type\">Definition<\/span><span class=\"space\"> <\/span><span class=\"codenumber\">5.2.1<\/span><span class=\"period\">.<\/span><\/h6><p id=\"p-659\">Let $T:V\\to V$ be a linear operator, and let $B=\\basis{b}{n}$ be an ordered basis of $V\\text{.}$ The matrix $M_B(T)=M_{BB}(T)$ is called the <dfn class=\"terminology\">$B$-matrix<\/dfn> of $T\\text{.}$<\/p><\/article><\/div>"]},
{"cell_type":"markdown", "metadata":{}, "source":["<div class=\"mathbook-content\"><p xmlns:svg=\"http:\/\/www.w3.org\/2000\/svg\" id=\"p-660\">The following result collects several useful properties of the $B$-matrix of an operator. Most of these were already encountered for the matrix $M_{DB}(T)$ of a transformation, although not all were stated formally. (Formal statements can be found in the textbook by Nicholson.)<\/p><\/div>"]},
{"cell_type":"markdown", "metadata":{}, "source":["<div class=\"mathbook-content\"><article class=\"theorem theorem-like\" id=\"thm-bmatrix-properties\"><h6 xmlns:svg=\"http:\/\/www.w3.org\/2000\/svg\" class=\"heading\"><span class=\"type\">Theorem<\/span><span class=\"space\"> <\/span><span class=\"codenumber\">5.2.2<\/span><span class=\"period\">.<\/span><\/h6><p id=\"p-661\">Let $T:V\\to V$ be a linear operator, and let $B=\\basis{b}{n}$ be a basis for $V\\text{.}$ Then<\/p><ol class=\"decimal\"><li id=\"li-121\">$C_B(T(\\vv))=M_B(T)C_B(\\vv)$ for all $\\vv\\in V\\text{.}$<\/li><li id=\"li-122\">If $S:V\\to V$ is another operator, then $M_B(ST)=M_B(S)M_B(T)\\text{.}$<\/li><li id=\"li-123\">$T$ is an isomorphism if and only if $M_B(T)$ is invertible.<\/li><li id=\"li-124\">If $T$ is an isomorphism, then $M_B(T^{-1}) = [M_B(T)]^{-1}\\text{.}$<\/li><li id=\"li-125\">$M_B(T)=\\bbm C_B(\\mathbf{b}_1) \\amp \\cdots \\amp C_B(\\mathbf{b}_n)\\ebm\\text{.}$<\/li><\/ol><\/article><\/div>"]},
{"cell_type":"markdown", "metadata":{}, "source":["<div class=\"mathbook-content\"><article class=\"example example-like\" id=\"example-9\"><h6 xmlns:svg=\"http:\/\/www.w3.org\/2000\/svg\" class=\"heading\"><span class=\"type\">Example<\/span><span class=\"space\"> <\/span><span class=\"codenumber\">5.2.3<\/span><span class=\"period\">.<\/span><\/h6><p id=\"p-662\">Find the $B$-matrix of the operator $T:P_2(\\R)\\to P_2(\\R)$ given by $T(p(x))=p(0)(1+x^2)+p(1)x\\text{,}$ with respect to the ordered basis<\/p><div class=\"displaymath\">\n\\begin{equation*}\nB = \\{1-x, x+3x^2, 2-x^2\\}\\text{.}\n\\end{equation*}\n<\/div><div class=\"solutions\"><a data-knowl=\"\" class=\"id-ref solution-knowl original\" data-refid=\"hk-solution-40\" id=\"solution-40\"><span class=\"type\">Solution<\/span><\/a><div class=\"hidden-content tex2jax_ignore\" id=\"hk-solution-40\"><div class=\"solution solution-like\"><p id=\"p-663\">We compute<\/p><div class=\"displaymath\">\n\\begin{align*}\nT(1-x) \\amp = 1(1+x^2)+0(x) = 1+x^2\\\\\nT(x+3x^2) \\amp = 0(1+x^2)+4x=4x\\\\\nT(2-x^2) \\amp = 2(1+x^2)+1(x) = 2+x+2x^2\\text{.}\n\\end{align*}\n<\/div><p class=\"continuation\">We now need to write each of these in terms of the basis $B\\text{.}$ We can do this by working out how to write each polynomial above in terms of $B\\text{.}$ Or we can be systematic.<\/p><p id=\"p-664\">Let $P = \\bbm 1\\amp 0\\amp 2\\\\-1\\amp 1\\amp 0\\\\0\\amp 3\\amp -1\\ebm$ be the matrix whose columns are given by the coefficient representations of the polynomials in $B$ with respect to the <em class=\"emphasis\">standard basis<\/em> $B_0=\\{1,x,x^2\\}\\text{.}$ For $T(1-x)=1+x^2$ we need to solve the equation<\/p><div class=\"displaymath\">\n\\begin{equation*}\na(1-x)+b(x+3x^2)+c(2-x^2)=1+x^2\n\\end{equation*}\n<\/div><p class=\"continuation\">for scalars $a,b,c\\text{.}$ But this is equivalent to the system<\/p><div class=\"displaymath\">\n\\begin{align*}\na+2c \\amp =1\\\\\n-a+b \\amp =0\\\\\n3b-c \\amp =1\\text{,}\n\\end{align*}\n<\/div><p class=\"continuation\">which, in turn, is equivalent to the matrix equation<\/p><div class=\"displaymath\">\n\\begin{equation*}\n\\bbm 1\\amp 0\\amp 2\\\\-1\\amp 1\\amp 0\\\\0\\amp 3\\amp -1\\ebm\\bbm a\\\\b\\\\c\\ebm = \\bbm 1\\\\0\\\\1\\ebm\\text{;}\n\\end{equation*}\n<\/div><p class=\"continuation\">that is, $PC_B(1+x^2) = C_{B_0}(1+x^2)\\text{.}$ Thus,<\/p><div class=\"displaymath\">\n\\begin{equation*}\nC_B(1+x^2) = \\bbm a\\\\b\\\\c\\ebm = P^{-1}C_{B_0}(1+x^2) = P^{-1}\\bbm 1\\\\0\\\\1\\ebm\\text{.}\n\\end{equation*}\n<\/div><p class=\"continuation\">Similarly, $C_B(4x)=P^{-1}\\bbm 0\\\\4\\\\0\\ebm = P^{-1}C_{B_0}(4x)\\text{,}$ and $C_B(2+x+2x^2)=P^{-1}\\bbm 2\\\\1\\\\2\\ebm = P^{-1}C_{B_0}(2+x+2x^2)\\text{.}$ Using the computer, we find:<\/p>{"cell_type":    "code", "execution_count":null, "metadata":{}, "source":["from sympy import *\ninit_printing()\nP = Matrix(3,3,[1,0,2,-1,1,0,0,3,-1])\nM = Matrix(3,3,[1,0,2,0,4,1,1,0,2])\nP**-1, P**-1*M"], "outputs":[]}<p id=\"p-665\">That is,<\/p><div class=\"displaymath\">\n\\begin{align*}\nM_B(T) \\amp =\\bbm C_B(T(1-x)) \\amp C_B(T(x+3x^2)) \\amp C_B(T(2-x^2))\\ebm\\\\\n\\amp =\\bbm P^{-1}C_{B_0}T(1-x) \\amp P^{-1} C_{B_0}T(x+3x^2) \\amp P^{-1}C_{B_0}(T(2-x^2))\\ebm\\\\\n\\amp =P^{-1}\\bbm C_{B_0}(1+x^2) \\amp C_{B_0}(4x)\\amp C_{B_0}(2+x+2x^2)\\ebm\\\\\n\\amp =\\bbm 1\/7\\amp -6\/7\\amp 3\/7\\\\1\/7\\amp 1\/7\\amp 2\/7\\\\3\/7\\amp 3\/7\\amp -1\/7\\ebm\n\\bbm 1\\amp 0\\amp 2\\\\0\\amp 4\\amp 1\\\\1\\amp 0\\amp 2\\ebm\\\\\n\\amp = \\bbm 3\/7\\amp -24\/7\\amp 0\\\\3\/7\\amp 4\/7\\amp 1\\\\2\/7\\amp 12\/7\\amp 1\\ebm\\text{.}\n\\end{align*}\n<\/div><p id=\"p-666\">Let's confirm that this works. Suppose we have<\/p><div class=\"displaymath\">\n\\begin{align*}\np(x) \\amp = C_B^{-1}\\bbm a\\\\b\\\\c\\ebm = a(1-x)+b(x+3x^2)+c(2-x^2)\\\\\n\\amp = (a+2c)+(-a+b)x+(3b-c)x^2\\text{.}\n\\end{align*}\n<\/div><p class=\"continuation\">Then $T(p(x))=(a+2c)(1+x^2)+(4b+c)x\\text{,}$ and we find<\/p><div class=\"displaymath\">\n\\begin{equation*}\nC_B(T(p(x))) = P^{-1}\\bbm a+2c\\\\4b+c\\\\a+2c\\ebm = \\bbm \\frac37 a-\\frac{24}{7}b\\\\\\frac37 a+\\frac47 b+c\\\\\\frac27 a+\\frac{12}{7}b+c\\ebm\\text{.}\n\\end{equation*}\n<\/div><p class=\"continuation\">On the other hand,<\/p><div class=\"displaymath\">\n\\begin{equation*}\nM_B(T) = \\bbm 3\/7\\amp -24\/7\\amp 0\\\\3\/7\\amp 4\/7\\amp 1\\\\2\/7\\amp 12\/7\\amp 1\\ebm\\bbm a\\\\b\\\\c\\ebm = \\bbm \\frac37 a-\\frac{24}{7}b\\\\\\frac37 a+\\frac47 b+c\\\\\\frac27 a+\\frac{12}{7}b+c\\ebm\\text{.}\n\\end{equation*}\n<\/div><p class=\"continuation\">The results agree, but possibly leave us a little confused.<\/p><\/div><\/div><\/div><\/article><\/div>"]},
{"cell_type":"markdown", "metadata":{}, "source":["<div class=\"mathbook-content\"><p id=\"p-667\">In general, given an ordered basis $B=\\basis{b}{n}$ for a vector space $V$ with standard basis $B_0 = \\basis{e}{n}\\text{,}$ if we let<\/p><div xmlns:svg=\"http:\/\/www.w3.org\/2000\/svg\" class=\"displaymath\">\n\\begin{equation*}\nP = \\bbm C_{B_0}(\\mathbf{b}_1) \\amp \\cdots \\amp C_{B_0}(\\mathbf{b}_n)\\ebm\\text{,}\n\\end{equation*}\n<\/div><p class=\"continuation\">then<\/p><div class=\"displaymath\">\n\\begin{align*}\nM_B(T) \\amp = \\bbm C_B(T(\\mathbf{b}_1)) \\amp \\cdots \\amp C_B(T(\\mathbf{b_n})\\ebm\\\\\n\\amp = P^{-1}\\bbm C_{B_0}(T(\\mathbf{b}_1)) \\amp \\cdots \\amp C_{B_0}(T(\\mathbf{b_n})\\ebm\\text{.}\n\\end{align*}\n<\/div><\/div>"]},
{"cell_type":"markdown", "metadata":{}, "source":["<div class=\"mathbook-content\"><p id=\"p-668\">As we saw above, this gives us the result, but doesn't shed much light on the problem, unless we have an easy way to write vectors in terms of the basis $B\\text{.}$ Let's revisit the problem. Instead of using the given basis $B\\text{,}$ let's use the standard basis $B_0 = \\{1,x,x^2\\}\\text{.}$ We quickly find<\/p><div xmlns:svg=\"http:\/\/www.w3.org\/2000\/svg\" class=\"displaymath\">\n\\begin{equation*}\nT(1)=1+x+x^2, T(x) = x, \\text{ and } T(x^2)=x\\text{,}\n\\end{equation*}\n<\/div><p class=\"continuation\">so with respect to the standard basis, $M_{B_0}(T) = \\bbm 1\\amp 0\\amp 0\\\\1\\amp 1\\amp 1\\\\1\\amp 0\\amp 0\\ebm\\text{.}$ Now, recall that<\/p><div class=\"displaymath\">\n\\begin{equation*}\nM_{B}(T)=P^{-1}\\bbm C_{B_0}T(1-x)\\amp C_{B_0}(T(x+3x^2)\\amp C_{B_0}(T(2-x^2))\\ebm\n\\end{equation*}\n<\/div><p class=\"continuation\">and note that for any polynomial $p(x)\\text{,}$ $C_{B_0}T(p(x)) = M_{B_0}C_{B_0}(p(x))\\text{.}$ But<\/p><div class=\"displaymath\">\n\\begin{equation*}\n\\bbm C_{B_0}(1-x) \\amp C_{B_0}(x+3x^2)\\amp C_{B_0}(2-x^2)\\ebm = P\\text{,}\n\\end{equation*}\n<\/div><p class=\"continuation\">so we get<\/p><div class=\"displaymath\">\n\\begin{align*}\nM_B(T) \\amp = P^{-1}\\bbm C_{B_0}T(1-x)\\amp C_{B_0}(T(x+3x^2)\\amp C_{B_0}(T(2-x^2))\\ebm\\\\\n\\amp = P^{-1}\\bbm M_{B_0}C_{B_0}(1-x)\\amp M_{B_0}C_{B_0}(x+3x^2)\\amp M_{B_0}C_{B_0}(2-x^2)\\ebm \\\\\n\\amp = P^{-1}M_{B_0}\\bbm C_{B_0}(1-x) \\amp C_{B_0}(x+3x^2)\\amp C_{B_0}(2-x^2)\\ebm\\\\\n\\amp = P^{-1}M_{B_0}P\\text{.}\n\\end{align*}\n<\/div><\/div>"]},
{"cell_type":"markdown", "metadata":{}, "source":["<div class=\"mathbook-content\"><p xmlns:svg=\"http:\/\/www.w3.org\/2000\/svg\" id=\"p-669\">Now we have a much more efficient method for arriving at the matrix $M_B(T)\\text{.}$ The matrix $M_{B_0}(T)$ is easy to determine, the matrix $P$ is easy to determine, and with the help of the computer, it's easy to compute $P^{-1}M_{B_0}P = M_B(T)\\text{.}$<\/p><\/div>"]},
{"cell_type":    "code", "execution_count":null, "metadata":{}, "source":["from sympy import *\ninit_printing()\nM0 = Matrix(3,3,[1,0,0,1,1,1,1,0,0])\nP**-1*M0*P"], "outputs":[]},
{"cell_type":"markdown", "metadata":{}, "source":["<div class=\"mathbook-content\"><article class=\"exercise exercise-like\" id=\"exercise-49\"><h6 xmlns:svg=\"http:\/\/www.w3.org\/2000\/svg\" class=\"heading\"><span class=\"type\">Exercise<\/span><span class=\"space\"> <\/span><span class=\"codenumber\">5.2.4<\/span><span class=\"period\">.<\/span><\/h6><p id=\"p-670\">Determine the matrix of the operator $T:\\R^3\\to \\R^3$ given by<\/p><div class=\"displaymath\">\n\\begin{equation*}\nT(x,y,z) = (3x-2y+4z,x-5y,2y-7z)\n\\end{equation*}\n<\/div><p class=\"continuation\">with respect to the ordered basis<\/p><div class=\"displaymath\">\n\\begin{equation*}\nB = \\{(1,2,0),(0,-1,2),(1,2,1)\\}\\text{.}\n\\end{equation*}\n<\/div><p class=\"continuation\">(You may want to use the Sage cell below for computational assistance.)<\/p><div class=\"solutions\"><a data-knowl=\"\" class=\"id-ref solution-knowl original\" data-refid=\"hk-solution-41\" id=\"solution-41\"><span class=\"type\">Solution<\/span><\/a><div class=\"hidden-content tex2jax_ignore\" id=\"hk-solution-41\"><div class=\"solution solution-like\"><p id=\"p-671\">With respect to the standard basis, we have<\/p><div class=\"displaymath\">\n\\begin{equation*}\nM_0=M_{B_0}(T) = \\bbm 3\\amp -2\\amp 4\\\\1\\amp -5\\amp 0\\\\0\\amp 2\\amp -7\\ebm\\text{,}\n\\end{equation*}\n<\/div><p class=\"continuation\">and the matrix $P$ is given by $P = \\bbm 1\\amp 3\\amp 1\\\\2\\amp -1\\amp 2\\\\0\\amp 2\\amp-5\\ebm\\text{.}$ Thus, we find<\/p><div class=\"displaymath\">\n\\begin{equation*}\nM_B(T)=P^{-1}M_0P=\\bbm 9\\amp 56\\amp 36\\\\7\\amp 15\\amp 15\\\\-10\\amp -46\\amp -33\\ebm\\text{.}\n\\end{equation*}\n<\/div><\/div><\/div><\/div><\/article><\/div>"]},
{"cell_type":    "code", "execution_count":null, "metadata":{}, "source":[""], "outputs":[]},
{"cell_type":"markdown", "metadata":{}, "source":["<div class=\"mathbook-content\"><p id=\"p-672\">The matrix $P$ used in the above examples is known as a <em xmlns:svg=\"http:\/\/www.w3.org\/2000\/svg\" class=\"emphasis\">change<\/em> matrix. If the columns of $P$ are the coefficient vectors of $B=\\basis{b}{n}$ with respect to another basis $D\\text{,}$ then we have<\/p><div class=\"displaymath\">\n\\begin{align*}\nP \\amp= \\bbm C_D(\\mathbf{b}_1)\\amp\\cdots \\amp C_D(\\mathbf{b}_n)\\ebm\\\\\n\\amp = \\bbm C_D(1_V(\\mathbf{b}_1))\\amp \\cdots \\amp C_D(1_V(\\mathbf{b}_n))\\ebm\\\\\n\\amp = M_{DB}(1_V)\\text{.}\n\\end{align*}\n<\/div><p class=\"continuation\">In other words, $P$ is the matrix of the identity transformation $1_V:V\\to V\\text{,}$ where we use the basis $B$ for the domain, and the basis $D$ for the codomain.<\/p><\/div>"]},
{"cell_type":"markdown", "metadata":{}, "source":["<div class=\"mathbook-content\"><article class=\"definition definition-like\" id=\"def-change-matrix\"><h6 xmlns:svg=\"http:\/\/www.w3.org\/2000\/svg\" class=\"heading\"><span class=\"type\">Definition<\/span><span class=\"space\"> <\/span><span class=\"codenumber\">5.2.5<\/span><span class=\"period\">.<\/span><\/h6><p id=\"p-673\">The <dfn class=\"terminology\">change matrix<\/dfn> with respect to ordered bases $B,D$ of $V$ is denoted $P_{D\\leftarrow B}\\text{,}$ and defined by<\/p><div class=\"displaymath\">\n\\begin{equation*}\nP_{D\\leftarrow B} = M_{DB}(1_V)\\text{.}\n\\end{equation*}\n<\/div><\/article><\/div>"]},
{"cell_type":"markdown", "metadata":{}, "source":["<div class=\"mathbook-content\"><article class=\"theorem theorem-like\" id=\"thm-change-matrix\"><h6 xmlns:svg=\"http:\/\/www.w3.org\/2000\/svg\" class=\"heading\"><span class=\"type\">Theorem<\/span><span class=\"space\"> <\/span><span class=\"codenumber\">5.2.6<\/span><span class=\"period\">.<\/span><\/h6><p id=\"p-674\">Let $B=\\basis{b}{n}$ and $D$ be two ordered bases of $V\\text{.}$ Then<\/p><div class=\"displaymath\">\n\\begin{equation*}\nP_{D\\leftarrow B} = \\bbm C_D(\\mathbf{b}_1)\\amp \\cdots \\amp C_D(\\mathbf{b}_n)\\ebm\\text{,}\n\\end{equation*}\n<\/div><p class=\"continuation\">and satisfies $C_D(\\vv) = P_{D\\leftarrow B}C_B(\\vv)$ for all $\\vv\\in V\\text{.}$<\/p><p id=\"p-675\">The matrix $P_{D\\leftarrow B}$ is invertible, and $(P_{D\\leftarrow B})^{-1} = P_{B\\leftarrow D}\\text{.}$ Moreover, if $E$ is a third ordered basis, then<\/p><div class=\"displaymath\">\n\\begin{equation*}\nP_{E\\leftarrow D}P_{D\\leftarrow B} = P_{E\\leftarrow B}\\text{.}\n\\end{equation*}\n<\/div><\/article><\/div>"]},
{"cell_type":"markdown", "metadata":{}, "source":["<div class=\"mathbook-content\"><article class=\"example example-like\" id=\"example-10\"><h6 xmlns:svg=\"http:\/\/www.w3.org\/2000\/svg\" class=\"heading\"><span class=\"type\">Example<\/span><span class=\"space\"> <\/span><span class=\"codenumber\">5.2.7<\/span><span class=\"period\">.<\/span><\/h6><p id=\"p-676\">Let $B = \\{1,x,x^2\\}$ and let $D = \\{1+x,x+x^2,2-3x+x^2\\}$ be ordered bases of $P_2(\\R)\\text{.}$ Find the change matrix $P_{D\\leftarrow B}\\text{.}$<\/p><div class=\"solutions\"><a data-knowl=\"\" class=\"id-ref solution-knowl original\" data-refid=\"hk-solution-42\" id=\"solution-42\"><span class=\"type\">Solution<\/span><\/a><div class=\"hidden-content tex2jax_ignore\" id=\"hk-solution-42\"><div class=\"solution solution-like\"><p id=\"p-677\">Finding this matrix requires us to first write the vectors in $B$ in terms of the vectors in $D\\text{.}$ However, it's much easier to do this the other way around. We easily find<\/p><div class=\"displaymath\">\n\\begin{equation*}\nP_{B\\leftarrow D} = \\bbm 1\\amp 0\\amp 2\\\\1\\amp 1\\amp -3\\\\0\\amp 1\\amp 1\\ebm\\text{,}\n\\end{equation*}\n<\/div><p class=\"continuation\">and by <a href=\"sec-matrix-operator.ipynb#thm-change-matrix\" class=\"internal\" title=\"Theorem 5.2.6\">Theorem 5.2.6<\/a>, we have<\/p><div class=\"displaymath\">\n\\begin{equation*}\nP_{D\\leftarrow B} = (P_{B\\leftarrow D})^{-1} = \\frac16\\bbm 4\\amp 2\\amp -2\\\\-1\\amp 1\\amp 5\\\\1\\amp -1\\amp 1\\ebm\\text{.}\n\\end{equation*}\n<\/div><\/div><\/div><\/div><\/article><\/div>"]},
{"cell_type":"markdown", "metadata":{}, "source":["<div class=\"mathbook-content\"><p id=\"p-678\">The above results give a straightforward procedure for determining the matrix of any operator, with respect to any basis, if we let $D$ be the standard basis. The importance of these results is not just their computational simplicity, however. The most important outcome of the above is that if $M_B(T)$ and $M_D(T)$ give the matrix of $T$ with respect to two different bases, then<\/p><div xmlns:svg=\"http:\/\/www.w3.org\/2000\/svg\" class=\"displaymath\">\n\\begin{equation*}\nM_B(T) = (P_{D\\leftarrow B})^{-1}M_B(T)P_{D\\leftarrow B}\\text{,}\n\\end{equation*}\n<\/div><p class=\"continuation\">so that the two matrices are <em class=\"emphasis\">similar<\/em>.<\/p><\/div>"]},
{"cell_type":"markdown", "metadata":{}, "source":["<div class=\"mathbook-content\"><p xmlns:svg=\"http:\/\/www.w3.org\/2000\/svg\" id=\"p-679\">Recall from <a href=\"subsec-eigen-basics.ipynb#thm-similar-properties\" class=\"internal\" title=\"Theorem 4.1.5\">Theorem 4.1.5<\/a> that similar matrices have the same determinant, trace, and eigenvalues. This means that we can unambiguously define the determinant and trace of an  <em class=\"emphasis\">operator<\/em>, and that we can compute eigenvalues of an operator using any matrix representation of that operator.<\/p><\/div>"]}
],
"nbformat": 4, "nbformat_minor": 0, "metadata": {"kernelspec": {"display_name": "", "name": "python3"}, "language_info": {"codemirror_mode": {"name": "ipython", "version": 3}, "file_extension": ".py", "mimetype": "text/x-python", "name": "python", "nbconvert_exporter": "python", "pygments_lexer": "ipython3", "version": "3.6.4"}, "name": "sec-matrix-operator.ipynb"}
}